Add weakening and substitution

structural.v
@@ -1,4 +1,4 @@
-From WR Require Import syntax join typing.
+From WR Require Import syntax join typing inversion.
 From Coq Require Import ssreflect.
 From Hammer Require Import Tactics.
 Require Import Psatz.
@@ -49,14 +49,83 @@ Qed.
 
 #[export]Hint Resolve wff_nil wff_cons : wff.
 
-Lemma renaming_Syn_mutual n Γ a A (h : Wt n Γ a A) : forall m Δ ξ,
+Lemma renaming_Syn n Γ a A (h : Wt n Γ a A) : forall m Δ ξ,
     good_renaming ξ n Γ m Δ ->
     Wff m Δ ->
     Wt m Δ (ren_tm ξ a) (ren_tm ξ A).
 Proof.
-  elim : Γ a A / h; try qauto l:on ctrs:Wt unfold:good_renaming.
+  elim : Γ a A / h; try qauto l:on depth:1 ctrs:Wt unfold:good_renaming.
   - hauto lq:on ctrs:Wt use:good_renaming_up db:wff.
-  - (* hauto lq:on ctrs:Wt use:good_renaming_up db:wff. *) admit.
+  - hauto lq:on ctrs:Wt use:good_renaming_up, Wt_Pi_Univ_inv db:wff.
   - move => * /=. apply : T_App'; eauto; by asimpl.
   - qauto l:on ctrs:Wt use:join_renaming.
-Admitted.
+Qed.
+
+Lemma Wt_Wff n Γ a A (h : Wt n Γ a A) : Wff n Γ.
+Proof. elim : Γ a A / h => //. Qed.
+
+#[export]Hint Resolve Wt_Wff : wff.
+
+Lemma weakening_Syn n Γ a A B i
+  (h0 : Wt n Γ B (tUniv i))
+  (h1 : Wt n Γ a A) :
+  Wt (S n) (B .: Γ) (ren_tm shift a) (ren_tm shift A).
+Proof.
+  apply renaming_Syn with (n := n) (Γ := Γ); eauto.
+  - split; [ rewrite /shift; lia | by rewrite dep_ith_ren_tm].
+  - hauto lq:on db:wff.
+Qed.
+
+Lemma weakening_Syn' n Γ a A A0 B i
+  (he : A0 = ren_tm shift A)
+  (h0 : Wt n Γ B (tUniv i))
+  (h1 : Wt n Γ a A) :
+  Wt (S n) (B .: Γ) (ren_tm shift a) A0.
+Proof. sfirstorder use:weakening_Syn. Qed.
+
+Definition good_morphing ρ n Γ m Δ :=
+  forall i, i < n -> Wt m Δ (ρ i) (subst_tm ρ (dep_ith Γ i)).
+
+Lemma T_Var' n Γ i A :
+  A = dep_ith Γ i ->
+  Wff n Γ ->
+  i < n ->
+  (* ------ *)
+  Wt n Γ (var_tm i) A.
+Proof. qauto ctrs:Wt. Qed.
+
+Lemma good_morphing_up ρ n k Γ m Δ A
+  (h : good_morphing ρ n Γ m Δ) :
+  Wff m Δ ->
+  Wt m Δ (subst_tm ρ A) (tUniv k) ->
+  good_morphing (up_tm_tm ρ) (S n) (A .: Γ) (S m) (subst_tm ρ A .: Δ).
+Proof.
+  rewrite /good_morphing => h1 h2.
+  case => [_ | i /Arith_prebase.lt_S_n ?].
+  - apply T_Var'.
+    + by asimpldep.
+    + eauto with wff.
+    + asimpl. lia.
+  - rewrite dep_ith_ren_tm.
+    apply : weakening_Syn'; cycle 2.
+    rewrite /good_morphing in h.
+    + sfirstorder unfold:good_morphing.
+    + by asimpl.
+    + sfirstorder.
+Qed.
+
+Lemma morphing_Syn n Γ a A (h : Wt n Γ a A) : forall m Δ ρ,
+    good_morphing ρ n Γ m Δ ->
+    Wff m Δ ->
+    Wt m Δ (subst_tm ρ a) (subst_tm ρ A).
+Proof.
+  elim : n Γ a A / h; try qauto l:on depth:1 ctrs:Wt unfold:good_morphing.
+  - move => *.
+    apply T_Pi; eauto.
+    hauto q:on use:good_morphing_up db:wff.
+  - move => *.
+    apply : T_Abs; eauto.
+    hauto q:on use:good_morphing_up, Wt_Pi_Univ_inv db:wff.
+  - move => * /=. apply : T_App'; eauto; by asimpl.
+  - hauto q:on ctrs:Wt use:join_subst_star.
+Qed.
